semantics_properties.v
@@ -4,568 +4,84 @@ Require Import Errors.
 Require Import more_stdlib function_utils spark2Cminor.
 Require Import Morphisms Relations.
 Import STACK.
+Import STACK.ST.
 
-Functional Scheme update_ind := Induction for update Sort Prop.
-Functional Scheme updates_ind := Induction for updates Sort Prop.
-Functional Scheme fetch_ind := Induction for fetch Sort Prop.
 
-Ltac rename_hyp1 h th :=
+(* Functional Scheme update_ind := Induction for update Sort Prop. *)
+(* Functional Scheme updates_ind := Induction for updates Sort Prop. *)
+(* Functional Scheme fetch_ind := Induction for fetch Sort Prop. *)
+
+Ltac rename_hyp_sem h th :=
   match th with
-    | in_bound _ _ _ => fresh "h_inbound"
-    | updates ?sto ?x _ = _ => fresh "heq_updates_" sto "_" x
-    | updates ?sto ?x _ = _ => fresh "heq_updates_" sto
-    | updates ?sto ?x _ = _ => fresh "heq_updates_" x
-    | updates ?sto ?x _ = _ => fresh "heq_updates"
-    | update ?frm ?x _ = _ => fresh "heq_update_" frm "_" x
-    | update ?frm ?x _ = _ => fresh "heq_update_" frm
-    | update ?frm ?x _ = _ => fresh "heq_update_" x
-    | update ?frm ?x _ = _ => fresh "heq_update"
-    | updateG ?stk ?x _ = _ => fresh "heq_updateG_" stk "_" x
-    | updateG ?stk ?x _ = _ => fresh "heq_updateG_" stk
-    | updateG ?stk ?x _ = _ => fresh "heq_updateG_" x
-    | updateG ?stk ?x _ = _ => fresh "heq_updateG"
-    | STACK.fetchG ?x ?stk = _ => fresh "heq_SfetchG_" x "_" stk
-    | STACK.fetchG ?x ?stk = _ => fresh "heq_SfetchG_" stk
-    | STACK.fetchG ?x ?stk = _ => fresh "heq_SfetchG_" x
-    | STACK.fetchG ?x ?stk = _ => fresh "heq_SfetchG"
-    | fetch ?x ?frm = _ => fresh "heq_fetch_" x "_" frm
-    | fetch ?x ?frm = _ => fresh "heq_fetch_" frm
-    | fetch ?x ?frm = _ => fresh "heq_fetch_" x
-    | fetch ?x ?frm = _ => fresh "heq_fetch"
-    | fetches ?x ?sto = _ => fresh "heq_fetches_" x "_" sto
-    | fetches ?x ?sto = _ => fresh "heq_fetches_" sto
-    | fetches ?x ?sto = _ => fresh "heq_fetches_" x
-    | fetches ?x ?sto = _ => fresh "heq_fetches"
-    | storeUpdate ?stbl ?s ?nme ?x (Normal ?rs) => fresh "h_storeUpd"
-    | storeUpdate ?stbl ?s ?nme ?x ?rs => fresh "h_storeUpd"
-    | fetch_var_type _ _ = Error _ => fresh "heq_fetch_var_type_ERR"
-    | fetch_var_type _ _ = _ => fresh "heq_fetch_var_type"
-    | spark2Cminor.compute_chnk _ ?name = OK ?chk => fresh "heq_compute_chnk_" name "_" chk
-    | spark2Cminor.compute_chnk _ ?name = ?chk => fresh "heq_compute_chnk_" name "_" chk
-    | spark2Cminor.compute_chnk _ ?name = _ => fresh "heq_compute_chnk_" name
-    | spark2Cminor.compute_chnk _ _ = _ => fresh "heq_compute_chnk"
-    | symboltable.fetch_exp_type _ _ = _ => fresh "heq_fetch_exp_type"
-    | symboltable.fetch_exp_type _ _ = Error _ => fresh "heq_fetch_exp_type_ERR"
-    | fetch_exp_type _ _ = None => fresh "heq_fetch_exp_type_none"
-    | fetch_exp_type _ _ = _ => fresh "heq_fetch_exp_type"
-    | eval_expr _ _ _ (Run_Time_Error _) => fresh "h_eval_expr_RE"
-    | eval_expr _ _ ?e (Normal ?v) => fresh "h_eval_expr_" e "_" v
-    | eval_expr _ _ _ (Normal ?v) => fresh "h_eval_expr_" v
-    | eval_expr _ _ ?e ?v => fresh "h_eval_expr_" e "_" v
-    | eval_expr _ _ ?e _ => fresh "h_eval_expr_" e
-    | eval_expr _ _ _ ?v => fresh "h_eval_expr_" v
-    | eval_expr _ _ _ _ => fresh "h_eval_expr"
-    | eval_name _ _ _ (Run_Time_Error _) => fresh "h_eval_name_RE"
-    | eval_name _ _ ?e (Normal ?v) => fresh "h_eval_name_" e "_" v
-    | eval_name _ _ _ (Normal ?v) => fresh "h_eval_name_" v
-    | eval_name _ _ ?e ?v => fresh "h_eval_name_" e "_" v
-    | eval_name _ _ ?e _ => fresh "h_eval_name_" e
-    | eval_name _ _ _ ?v => fresh "h_eval_name_" v
-    | eval_name _ _ _ _ => fresh "h_eval_name"
-    | do_overflow_check _ (Run_Time_Error _) => fresh "h_overf_check_RE"
-    | do_overflow_check _ _ => fresh "h_overf_check"
-    | do_range_check _ _ _ (Run_Time_Error _) => fresh "h_do_range_check_RE"
-    | do_range_check _ _ _ _ => fresh "h_do_range_check"
-    | do_run_time_check_on_binop _ _ _ (Run_Time_Error _) => fresh "h_do_rtc_binop_RTE"
-    | do_run_time_check_on_binop _ _ _ _ => fresh "h_do_rtc_binop"
-    | eval_literal _ (Run_Time_Error _)  => fresh "h_eval_literal_RE"
-    | eval_literal _ _  => fresh "h_eval_literal"
-    | eval_stmt _ _ _ (Run_Time_Error _) => fresh "h_eval_stmt_RE"
-    | eval_stmt _ _ _ _ => fresh "h_eval_stmt"
-    | eval_decl _ _ _ _ (Run_Time_Error _) => fresh "h_eval_stmt_RE"
-    | eval_decl _ _ _ _ _ => fresh "h_eval_stmt"
-    | storeUpdate _ _ _ _ (Run_Time_Error _) => fresh "h_storeupdate_RTE"
-    | storeUpdate _ _ _ _ _ => fresh "h_storeupdate"
-    | do_run_time_check_on_binop _ _ _ (Run_Time_Error _) =>  fresh "h_do_rtc_binop_RE"
-    | do_run_time_check_on_binop _ _ _ _ =>  fresh "h_do_rtc_binop"
-    | do_run_time_check_on_unop _ _ (Run_Time_Error _) =>  fresh "h_do_rtc_unop_RE"
-    | do_run_time_check_on_unop _ _ _ =>  fresh "h_do_rtc_unop"
-    | do_division_check _ _ (Run_Time_Error _) => fresh "h_do_division_check_RTE"
-    | do_division_check _ _ _ => fresh "h_do_division_check"
-    | extract_subtype_range _ ?t ?rge => fresh "subtype_rge_" t "_" rge
-    | extract_subtype_range _ ?t _ => fresh "subtype_rge_" t
-    | extract_subtype_range _ _ _ => fresh "subtype_rge"
-    | copy_out ?st ?s ?pstmt ?paramsprf ?args (Run_Time_Error ?er) => fresh "h_copy_out_RE"
-    | copy_out ?st ?s ?pstmt ?paramsprf ?args (Normal ?s') => fresh "h_copy_out_" s "_" s'
-    | copy_out ?st ?s ?pstmt ?paramsprf ?args ?s' => fresh "h_copy_out_" s "_" s'
-    | copy_out ?st ?s ?pstmt ?paramsprf ?args _ => fresh "h_copy_out_" s
-    | copy_out ?st ?s ?pstmt ?paramsprf ?args _ => fresh "h_copy_out"
+  | fetch_var_type _ _ = Error _ => fresh "heq_fetch_var_type_ERR"
+  | fetch_var_type _ _ = _ => fresh "heq_fetch_var_type"
+  | spark2Cminor.compute_chnk _ ?name = OK ?chk => fresh "heq_compute_chnk_" name "_" chk
+  | spark2Cminor.compute_chnk _ ?name = ?chk => fresh "heq_compute_chnk_" name "_" chk
+  | spark2Cminor.compute_chnk _ ?name = _ => fresh "heq_compute_chnk_" name
+  | spark2Cminor.compute_chnk _ _ = _ => fresh "heq_compute_chnk"
+  | symboltable.fetch_exp_type _ _ = _ => fresh "heq_fetch_exp_type"
+  | symboltable.fetch_exp_type _ _ = Error _ => fresh "heq_fetch_exp_type_ERR"
+  | fetch_exp_type _ _ = None => fresh "heq_fetch_exp_type_none"
+  | fetch_exp_type _ _ = _ => fresh "heq_fetch_exp_type"
+  | eval_expr _ _ _ (Run_Time_Error _) => fresh "h_eval_expr_RE"
+  | eval_expr _ _ ?e (Normal ?v) => fresh "h_eval_expr_" e "_" v
+  | eval_expr _ _ _ (Normal ?v) => fresh "h_eval_expr_" v
+  | eval_expr _ _ ?e ?v => fresh "h_eval_expr_" e "_" v
+  | eval_expr _ _ ?e _ => fresh "h_eval_expr_" e
+  | eval_expr _ _ _ ?v => fresh "h_eval_expr_" v
+  | eval_expr _ _ _ _ => fresh "h_eval_expr"
+  | eval_name _ _ _ (Run_Time_Error _) => fresh "h_eval_name_RE"
+  | eval_name _ _ ?e (Normal ?v) => fresh "h_eval_name_" e "_" v
+  | eval_name _ _ _ (Normal ?v) => fresh "h_eval_name_" v
+  | eval_name _ _ ?e ?v => fresh "h_eval_name_" e "_" v
+  | eval_name _ _ ?e _ => fresh "h_eval_name_" e
+  | eval_name _ _ _ ?v => fresh "h_eval_name_" v
+  | eval_name _ _ _ _ => fresh "h_eval_name"
+  | do_overflow_check _ (Run_Time_Error _) => fresh "h_overf_check_RE"
+  | do_overflow_check _ _ => fresh "h_overf_check"
+  | do_range_check _ _ _ (Run_Time_Error _) => fresh "h_do_range_check_RE"
+  | do_range_check _ _ _ _ => fresh "h_do_range_check"
+  | do_run_time_check_on_binop _ _ _ (Run_Time_Error _) => fresh "h_do_rtc_binop_RTE"
+  | do_run_time_check_on_binop _ _ _ _ => fresh "h_do_rtc_binop"
+  | eval_literal _ (Run_Time_Error _)  => fresh "h_eval_literal_RE"
+  | eval_literal _ _  => fresh "h_eval_literal"
+  | eval_stmt _ _ _ (Run_Time_Error _) => fresh "h_eval_stmt_RE"
+  | eval_stmt _ _ _ _ => fresh "h_eval_stmt"
+  | eval_decl _ _ _ _ (Run_Time_Error _) => fresh "h_eval_stmt_RE"
+  | eval_decl _ _ _ _ _ => fresh "h_eval_stmt"
+  | storeUpdate _ _ _ _ (Run_Time_Error _) => fresh "h_storeUpd_RE"
+  | storeUpdate _ _ _ _ _ => fresh "h_storeUpd"
+  | do_run_time_check_on_binop _ _ _ (Run_Time_Error _) =>  fresh "h_do_rtc_binop_RE"
+  | do_run_time_check_on_binop _ _ _ _ =>  fresh "h_do_rtc_binop"
+  | do_run_time_check_on_unop _ _ (Run_Time_Error _) =>  fresh "h_do_rtc_unop_RE"
+  | do_run_time_check_on_unop _ _ _ =>  fresh "h_do_rtc_unop"
+  | do_division_check _ _ (Run_Time_Error _) => fresh "h_do_division_check_RTE"
+  | do_division_check _ _ _ => fresh "h_do_division_check"
+  | extract_subtype_range _ ?t ?rge => fresh "subtype_rge_" t "_" rge
+  | extract_subtype_range _ ?t _ => fresh "subtype_rge_" t
+  | extract_subtype_range _ _ _ => fresh "subtype_rge"
+  | copy_out ?st ?s ?pstmt ?paramsprf ?args (Run_Time_Error ?er) => fresh "h_copy_out_RE"
+  | copy_out ?st ?s ?pstmt ?paramsprf ?args (Normal ?s') => fresh "h_copy_out_" s "_" s'
+  | copy_out ?st ?s ?pstmt ?paramsprf ?args ?s' => fresh "h_copy_out_" s "_" s'
+  | copy_out ?st ?s ?pstmt ?paramsprf ?args _ => fresh "h_copy_out_" s
+  | copy_out ?st ?s ?pstmt ?paramsprf ?args _ => fresh "h_copy_out"
 
-    | copy_in ?st ?s ?fr ?paramsprf ?args (Run_Time_Error ?er) => fresh "h_copy_in_RE"
-    | copy_in ?st ?s ?fr ?paramsprf ?args (Normal ?fr') => fresh "h_copy_in_" fr "_" fr'
-    | copy_in ?st ?s ?fr ?paramsprf ?args ?fr' => fresh "h_copy_in_" fr "_" fr'
-    | copy_in ?st ?s ?fr ?paramsprf ?args _ => fresh "h_copy_in_" fr
-    | copy_in ?st ?s ?fr ?paramsprf ?args _ => fresh "h_copy_in"
-    | cut_until ?st ?s ?fr ?paramsprf ?args (Run_Time_Error ?er) => fresh "h_cut_until_RE"
-    | cut_until ?st ?s ?fr ?paramsprf ?args (Normal ?fr') => fresh "h_cut_until_" fr "_" fr'
-    | cut_until ?st ?s ?fr ?paramsprf ?args ?fr' => fresh "h_cut_until_" fr "_" fr'
-    | cut_until ?st ?s ?fr ?paramsprf ?args _ => fresh "h_cut_until_" fr
-    | cut_until ?st ?s ?fr ?paramsprf ?args _ => fresh "h_cut_until"
+  | copy_in ?st ?s ?fr ?paramsprf ?args (Run_Time_Error ?er) => fresh "h_copy_in_RE"
+  | copy_in ?st ?s ?fr ?paramsprf ?args (Normal ?fr') => fresh "h_copy_in_" fr "_" fr'
+  | copy_in ?st ?s ?fr ?paramsprf ?args ?fr' => fresh "h_copy_in_" fr "_" fr'
+  | copy_in ?st ?s ?fr ?paramsprf ?args _ => fresh "h_copy_in_" fr
+  | copy_in ?st ?s ?fr ?paramsprf ?args _ => fresh "h_copy_in"
 
-    | symboltable.fetch_proc ?p _ = None => fresh "h_fetch_proc_None_" p
-    | symboltable.fetch_proc _ _ = None => fresh "h_fetch_proc_None"
-    | symboltable.fetch_proc ?p _ = Some ?r => fresh "h_fetch_proc_" p "_" r
-    | symboltable.fetch_proc ?p _ = ?r => fresh "h_fetch_proc_" p "_" r
-    | symboltable.fetch_proc ?p _ = _ => fresh "h_fetch_proc_" p
-    | symboltable.fetch_proc _ _ = _ => fresh "h_fetch_proc"
+  | symboltable.fetch_proc ?p _ = None => fresh "h_fetch_proc_None_" p
+  | symboltable.fetch_proc _ _ = None => fresh "h_fetch_proc_None"
+  | symboltable.fetch_proc ?p _ = Some ?r => fresh "h_fetch_proc_" p "_" r
+  | symboltable.fetch_proc ?p _ = ?r => fresh "h_fetch_proc_" p "_" r
+  | symboltable.fetch_proc ?p _ = _ => fresh "h_fetch_proc_" p
+  | symboltable.fetch_proc _ _ = _ => fresh "h_fetch_proc"
+  | _ => STACK.rename_hyp1 h th
   end.
 
-Ltac rename_hyp ::= rename_hyp1.
-
-
-Lemma updates_ok_none : forall sto x v, updates sto x v = None <-> fetches x sto = None.
-Proof.
-  !intros.
-  split;!intro.
-  - !functional induction (updates sto x v).
-    + discriminate.
-    + discriminate.
-    + unfold id in *. (* scorie from libhyprenaming *)
-      simpl.
-      rewrite hbeqnat_false.
-      apply IHo.
-      assumption.
-    + reflexivity.
-  - !functional induction (fetches x sto).
-    + discriminate.
-    + unfold id in *. (* scorie from libhyprenaming *)
-      simpl.
-      rewrite hbeqnat_false.
-      rewrite IHo;auto.
-    + reflexivity.
-Qed.
-
-(* the none version could be solved by functiona inversion but it is
-   ot applicable here due to a bug in Function with functors. *)
-Lemma update_ok_none : forall frm x v, update frm x v = None <-> fetch x frm = None.
-Proof.
-  !intros.
-  split.
-  - !functional induction (update frm x v);!intro.
-    + discriminate.
-    + unfold fetch.
-      eapply updates_ok_none;eauto.
-  - unfold fetch, update.
-    !intro.
-    rewrite <- updates_ok_none in heq_fetches_x.
-    rewrite heq_fetches_x.
-    reflexivity.
-Qed.
-
-
-(* the none version could be solved by functiona inversion but it is
-   ot applicable here due to a bug in Function with functors. *)
-Lemma updateG_ok_none : forall stk x v, updateG stk x v = None <-> fetchG x stk = None.
-Proof.
-  !intros.
-  split.
-  - !functional induction (updateG stk x v);!intro.
-    + discriminate.
-    + discriminate.
-    + unfold id in *.
-      simpl.
-      apply update_ok_none in heq_update_f_x.
-      rewrite heq_update_f_x.
-      auto.
-    + reflexivity.
-  - !functional induction (fetchG x stk);!intro.
-    + discriminate.
-    + simpl.
-      rewrite IHo;auto.
-      rewrite <- update_ok_none in heq_fetch_x_f;eauto.
-      rewrite heq_fetch_x_f;auto.
-   + reflexivity.
-Qed.
-
-Lemma fetches_ok: forall id sto v, fetches id sto = Some v -> resides id sto = true.
-Proof.
-  intros id sto v.
-  !functional induction (fetches id sto);!intros;try discriminate.
-  - inversion heq.
-    subst.
-    cbn.
-    rewrite hbeqnat_true.
-    reflexivity.
-  - cbn.
-    rewrite hbeqnat_false.
-    auto.
-Qed.
-
-Lemma compilenv_fetches_resides: forall nme x,
-    (exists res, CompilEnv.fetches nme x = Some res) <->
-    CompilEnv.resides nme x = true.
-Proof.
-  !!intros ? ?.
-  !functional induction (CompilEnv.fetches nme x);cbn;!intros;subst.
-  - rewrite hbeqnat_true.
-    split;eauto.
-  - rewrite hbeqnat_false.
-    assumption.
-  - split;!intros; try discriminate.
-    decompose [ex] h_ex.
-    discriminate.
-Qed.
-
-
-Lemma fetches_ok_none: forall id sto, fetches id sto = None -> resides id sto = false.
-Proof.
-  intros id sto.
-  !functional induction (fetches id sto);!intros;try discriminate.
-  - cbn.
-    rewrite hbeqnat_false.
-    auto.
-  - cbn.
-    reflexivity.
-Qed.
-
-Lemma fetch_ok: forall id sto v, fetch id sto = Some v -> reside id sto = true.
-Proof.
-  unfold fetch, reside.
-  !intros.
-  apply fetches_ok in heq_fetches_id.
-  assumption.
-Qed.
-
-Lemma fetch_ok_none: forall id sto, fetch id sto = None -> reside id sto = false.
-Proof.
-  unfold fetch, reside.
-  !intros.
-  apply fetches_ok_none in heq_fetches_id.
-  assumption.
-Qed.
-
-Lemma fetchG_ok_none: forall id sto, fetchG id sto = None -> resideG id sto = false.
-Proof.
-  intros id sto.
-  !functional induction (fetchG id sto);!intros;try discriminate.
-  - simpl.
-    !!destruct (reside id f) eqn:heq_reside.
-    + apply fetch_ok_none in heq_fetch_id_f.
-      rewrite heq_fetch_id_f in heq_bool_true;discriminate.
-    + auto.
-  - reflexivity. 
-Qed.
-
-Lemma fetchG_ok: forall id sto v, fetchG id sto = Some v -> resideG id sto = true.
-Proof.
-  intros id sto.
-  !functional induction (fetchG id sto);!intros;try discriminate.
-  - simpl.
-    !!destruct (reside id f) eqn:heq_reside.
-    + reflexivity.
-    + apply fetch_ok in heq_fetch_id_f.
-      rewrite heq_fetch_id_f in heq_bool_false;discriminate.
-  - simpl.
-    !!destruct (reside id f) eqn:heq_reside.
-    + reflexivity.
-    + apply IHo in heq_SfetchG_id_s'.
-      assumption.
-Qed.
-
-Lemma updates_ok_same: forall sto id v sto',
-    updates sto id v = Some sto'
-    -> fetches id sto' = Some v.
-Proof.
-  intros until v.
-  !functional induction (updates sto id v);!intros;simpl in *;intros.
-  - !invclear heq;simpl.
-    rewrite hbeqnat_true.
-    reflexivity.
-  - !invclear heq;simpl.
-    !invclear heq_updates_s'_x;simpl.
-    rewrite hbeqnat_false.
-    apply IHo.
-    assumption.
-  - discriminate.
-  - discriminate.
-Qed.
-
-Lemma updates_ok_same_orig: forall sto id v sto',
-    updates sto id v = Some sto'
-    -> exists v', fetches id sto = Some v'.
-Proof.
-  intros sto id v.
-  !functional induction (updates sto id v);!intros;simpl in *;intros.
-  - rewrite hbeqnat_true.
-    eauto.
-  - rewrite hbeqnat_false.
-    eapply IHo;eauto.
-  - discriminate.
-  - discriminate.
-Qed.
-
-Lemma updates_ok_same_resides: forall sto id v sto',
-    updates sto id v = Some sto'
-    -> resides id sto' = true.
-Proof.
-  !intros.
-  eapply fetches_ok.
-  eapply updates_ok_same;eauto.
-Qed.
-
-Lemma updates_ok_same_resides_orig: forall sto id v sto',
-    updates sto id v = Some sto'
-    -> resides id sto = true.
-Proof.
-  !intros.
-  !!pose proof updates_ok_same_orig _ _ _ _ heq_updates_sto_id.
-  destruct h_ex.
-  eapply fetches_ok;eauto.
-Qed.
-
-Lemma update_ok_same: forall frm id v frm',
-    update frm id v = Some frm'
-    -> fetch id frm' = Some v.
-Proof.
-  intros until v.
-  unfold fetch, update.
-  !intros.
-  destruct (updates (store_of frm) id v) eqn:heq_upd.
-  - !invclear heq;simpl.
-    eapply updates_ok_same;eauto.
-  - discriminate.
-Qed.
-
-
-Lemma update_ok_same_orig: forall frm id v frm',
-    update frm id v = Some frm'
-    -> exists v', fetch id frm = Some v'.
-Proof.
-  intros until v.
-  unfold fetch, update.
-  !intros.
-  destruct (updates (store_of frm) id v) eqn:heq_upd.
-  - !invclear heq;simpl.
-    !!pose proof updates_ok_same_orig _ _ _ _ heq_upd.
-    assumption.
-  - discriminate.
-Qed.
-
-Lemma update_ok_same_reside: forall sto id v sto',
-    update sto id v = Some sto'
-    -> reside id sto' = true.
-Proof.
-  !intros.
-  eapply fetch_ok.
-  eapply update_ok_same;eauto.
-Qed.
-
-Lemma update_ok_same_reside_orig: forall sto id v sto',
-    update sto id v = Some sto'
-    -> reside id sto = true.
-Proof.
-  !intros.
-  !!pose proof update_ok_same_orig _ _ _ _ heq_update_sto_id.
-  destruct h_ex.
-  eapply fetch_ok;eauto.
-Qed.
-
-Lemma updateG_ok_same: forall stk id v stk',
-    updateG stk id v = Some stk'
-    -> fetchG id stk' = Some v.
-Proof.
-  intros until v.
-  !functional induction (updateG stk id v);simpl;!intros.
-  - !invclear heq;simpl.
-    apply update_ok_same in heq_update_f_x.
-    rewrite heq_update_f_x.
-    reflexivity.
-  - !invclear heq;simpl.
-    specialize (IHo _ heq_updateG_s'_x).
-    destruct (fetch x f) eqn:h.
-    + apply update_ok_none in heq_update_f_x.
-      rewrite heq_update_f_x in h;discriminate.
-    + assumption.
-  - discriminate.
-  - discriminate.
-Qed.
-
-Lemma updateG_ok_same_orig: forall stk id v stk',
-    updateG stk id v = Some stk'
-    -> exists v', fetchG id stk = Some v'.
-Proof.
-  intros until v.
-  !functional induction (updateG stk id v);simpl;!intros;try discriminate.
-  - !invclear heq;simpl.
-    !destruct (update_ok_same_orig _ _ _ _ heq_update_f_x).
-    rewrite heq_fetch_x_f.
-    eauto.
-  - !invclear heq;simpl.
-    apply update_ok_none in heq_update_f_x.
-    rewrite heq_update_f_x.
-    eapply IHo.
-    eauto.
-Qed.
-
-Lemma updateG_ok_same_resideG: forall stk id v stk',
-    updateG stk id v = Some stk'
-    -> resideG id stk' = true.
-Proof.
-  !intros.
-  eapply fetchG_ok.
-  eapply updateG_ok_same.
-  eauto.
-Qed.
-
-
-
-Lemma updates_ok_others: forall sto id v sto',
-    updates sto id v = Some sto' ->
-    forall id', id<>id' -> fetches id' sto = fetches id' sto'.
-Proof.
-  intros until v.
-  !functional induction (updates sto id v);!intros;simpl in *;intros.
-  - !invclear heq;simpl.
-    rewrite -> Nat.eqb_eq in hbeqnat_true.
-    subst.
-    apply Nat.neq_sym in hneq.
-    rewrite <- Nat.eqb_neq in hneq.
-    rewrite hneq in *.
-    reflexivity.
-  - !invclear heq;simpl.
-    destruct (Nat.eq_dec id' y).
-    + subst.
-      rewrite Nat.eqb_refl in *.
-      reflexivity.
-    + rewrite <- Nat.eqb_neq in n.
-      rewrite n in *.
-      eapply IHo;eauto.
-  - discriminate.
-  - discriminate.
-Qed.
-
-Lemma update_ok_others: forall frm id v frm',
-    update frm id v = Some frm' ->
-    forall id', id<>id' -> fetch id' frm = fetch id' frm'.
-Proof.
-  intros until v.
-  !functional induction (STACK.update frm id v);!destruct frm;simpl in *;!intros.
-  - !invclear heq;simpl.
-    eapply updates_ok_others in heq_updates_id;eauto.
-  - discriminate.
-Qed.
-
-Lemma update_ok_others_reside: forall frm id v frm',
-    update frm id v = Some frm' ->
-    forall id', id<>id' -> reside id' frm = reside id' frm'.
-Proof.
-  !intros.
-  !!pose proof update_ok_others _ _ _ _ heq_update_frm_id _ hneq.
-  destruct (fetch id' frm) eqn:heq_fetch.
-  - apply fetch_ok in heq_fetch.
-    rewrite heq_fetch.
-    symmetry in heq_fetch_id'_frm.
-    apply fetch_ok in heq_fetch_id'_frm.
-    rewrite heq_fetch_id'_frm.
-    reflexivity.
-  - apply fetch_ok_none in heq_fetch.
-    rewrite heq_fetch.
-    symmetry in heq_fetch_id'_frm.
-    apply fetch_ok_none in heq_fetch_id'_frm.
-    rewrite heq_fetch_id'_frm.
-    reflexivity.
-Qed.
-
-Lemma updateG_ok_others: forall stk id v stk',
-    updateG stk id v = Some stk' ->
-    forall id', id<>id' -> fetchG id' stk = fetchG id' stk'.
-Proof.
-  intros until v.
-  !functional induction (updateG stk id v);simpl;!intros.
-  - !invclear heq;simpl.
-    !! (destruct (fetch id' f) eqn:h).
-    + erewrite update_ok_others in heq_fetch_id'_f;eauto.
-      rewrite heq_fetch_id'_f.
-      reflexivity.
-    + erewrite update_ok_others in heq_fetch_id'_f;eauto.
-      rewrite heq_fetch_id'_f.
-      reflexivity.
-  - !invclear heq;simpl.
-    !! (destruct (fetch id' f) eqn:h).
-    + reflexivity.
-    + eapply IHo;eauto.
-  - discriminate.
-  - discriminate.
-Qed.
-
-
-Lemma updateG_ok_others_resideG: forall frm id v frm',
-    updateG frm id v = Some frm' ->
-    forall id', id<>id' -> resideG id' frm = resideG id' frm'.
-Proof.
-  !intros.
-  !!pose proof updateG_ok_others _ _ _ _ heq_updateG_frm_id _ hneq.
-  destruct (fetchG id' frm) eqn:heq_fetchG.
-  - apply fetchG_ok in heq_fetchG.
-    rewrite heq_fetchG.
-    symmetry in heq_SfetchG_id'_frm.
-    apply fetchG_ok in heq_SfetchG_id'_frm.
-    rewrite heq_SfetchG_id'_frm.
-    reflexivity.
-  - apply fetchG_ok_none in heq_fetchG.
-    rewrite heq_fetchG.
-    symmetry in heq_SfetchG_id'_frm.
-    apply fetchG_ok_none in heq_SfetchG_id'_frm.
-    rewrite heq_SfetchG_id'_frm.
-    reflexivity.
-Qed.
-
-
-Lemma updateG_ok_same_frameG: forall stk id v lvl sto stk',
-    updateG stk id v = Some stk'
-    -> frameG id stk = Some (lvl,sto)
-    -> exists sto', frameG id stk' = Some (lvl,sto').
-Proof.
-  intros until v.
-  !functional induction (updateG stk id v);simpl;!intros;try discriminate.
-  - !invclear heq;simpl.
-    !!pose proof update_ok_same_reside _ _ _ _ heq_update_f_x.
-    !!pose proof update_ok_same_reside_orig _ _ _ _ heq_update_f_x.
-    rewrite heq_bool_true.
-    rewrite heq_bool_true0 in heq0.
-    !invclear heq0.
-    unfold update in heq_update_f_x.
-    cbn in *.
-    destruct (updates sto x v) eqn:heq.
-    + eauto.
-    + discriminate.
-  - !invclear heq;simpl.
-    rewrite update_ok_none in heq_update_f_x.
-    apply fetch_ok_none in heq_update_f_x.
-    rewrite heq_update_f_x.
-    rewrite heq_update_f_x in heq0.
-    eauto.
-Qed.
-
-Lemma updateG_ok_same_frameG_orig: forall stk id v lvl sto stk',
-    updateG stk id v = Some stk'
-    -> frameG id stk' = Some (lvl,sto)
-    -> exists sto', frameG id stk = Some (lvl,sto').
-Proof.
-  intros until v.
-  !functional induction (updateG stk id v);simpl;!intros;try discriminate.
-  - !invclear heq;simpl.
-    !!pose proof update_ok_same_reside _ _ _ _ heq_update_f_x.
-    !!pose proof update_ok_same_reside_orig _ _ _ _ heq_update_f_x.
-    simpl in heq0.
-    rewrite heq_bool_true in heq0.
-    rewrite heq_bool_true0.
-    !invclear heq0.
-    unfold update in heq_update_f_x.
-    cbn in *.
-    destruct (updates (store_of f) x v) eqn:heq.
-    + destruct f;simpl in *.
-      !invclear heq_update_f_x.
-      eauto.
-    + discriminate.
-  - !invclear heq;simpl.
-    simpl in heq0.
-    rewrite update_ok_none in heq_update_f_x.
-    apply fetch_ok_none in heq_update_f_x.
-    rewrite heq_update_f_x.
-    rewrite heq_update_f_x in heq0.
-    eapply IHo; eauto.
-Qed.
+Ltac rename_hyp ::= rename_hyp_sem.
 
 Lemma storeUpdate_id_ok_others: forall ast_num stbl stk id v stk',
     storeUpdate stbl stk (E_Identifier ast_num id) v (Normal stk') ->
@@ -656,7 +172,7 @@ Proof.
     reflexivity.
 Qed.
 
-Set Printing Width 120.
+
 
 Lemma arrayUpdate_id_ok_others: forall arr k v arr',
     arrayUpdate (ArrayV arr) k v = Some (ArrayV arr')
@@ -683,7 +199,7 @@ Inductive follow_chaining: Values.val -> Memory.Mem.mem -> nat -> Values.val -> 
     frame [sto]. *)
 (* FIXME: are we looking at the stack in the wrong direction? *)
 Inductive eq_frame:
-  STACK.store -> Values.block -> Integers.Int.int -> Memory.Mem.mem -> Prop :=
+  store -> Values.block -> Integers.Int.int -> Memory.Mem.mem -> Prop :=
   MF1: forall spb ofs m, eq_frame nil spb ofs m
 | MF2: forall fr spb ofs m id vid t_vid,
     Memory.Mem.load AST.Mint32 m spb ofs = Some t_vid ->
@@ -695,9 +211,9 @@ Inductive eq_frame:
 (** [match_env sta b m] means that the chained Cminor stack at address
     [b] in memory m ([b] is the adress of the bottom of the top stack)
     matches spark stack [s]. *)
-Inductive eq_env: STACK.stack -> Values.block -> Memory.Mem.mem -> Prop :=
+Inductive eq_env: stack -> Values.block -> Memory.Mem.mem -> Prop :=
   ME1: forall spb m, eq_env nil spb m
-| ME2: forall s sto (lvl:STACK.scope_level) fr spb spb' m,
+| ME2: forall s sto (lvl:scope_level) fr spb spb' m,
          eq_frame fr spb (Integers.Int.repr 4) m
          -> eq_env s spb' m
          -> eq_env ((lvl,sto)::s) spb m.
